\newpage
\section{Chapter 10}

\begin{problem} \notfinish
\end{problem}

\begin{problem} \notfinish
\end{problem}

\begin{problem} This follows from the direct computation:
\begin{align*}
    &E(x, I(\sigma, \lambda)(g)\varphi, \lambda) \\
    &= \sum_{\delta \in P(F) \backslash G(F)} I(\sigma, \lambda)(g)\varphi(\delta x)
    e^{\langle H_P(\delta x), \lambda + \rho_P \rangle} \\
    &= \sum_{\delta \in P(F) \backslash G(F)} \varphi(\delta x g ) e^{\langle H_P(\delta x g), \lambda + \rho_P \rangle}e^{-\langle H_P(\delta x), \lambda + \rho_P \rangle} e^{\langle H_P(\delta x), \lambda + \rho_P \rangle}\\
    &= \sum_{\delta \in P(F) \backslash G(F)} \varphi(\delta x g ) e^{\langle H_P(\delta x g), \lambda + \rho_P \rangle} \\
    &= E(xg, \varphi, \lambda).
\end{align*}
\end{problem}

\begin{problem} \notfinish
\end{problem}

\begin{problem} \notfinish
\end{problem}

\begin{problem} \notfinish
\end{problem}

\begin{problem} \notfinish
\end{problem}

\begin{problem} \notfinish
\end{problem}

\begin{problem} \notfinish
\end{problem}